src/rocq_ind.ml
@@ -47,14 +47,14 @@ let to_string
 
 (***********************************************************************)
 
-exception Rocq_ind_UnexpectedKind of kind
+exception UnexpectedKind of kind
 
 let get_lts ({ kind; _ } : 'a t) : LTS.t =
   Log.trace __FUNCTION__;
   match kind with
   | LTS l -> l
   (* | _ -> invalid_cindef_kind () *)
-  | x -> raise (Rocq_ind_UnexpectedKind x)
+  | x -> raise (UnexpectedKind x)
 ;;
 
 let get_lts_term_type (x : 'a t) : EConstr.t =
@@ -88,8 +88,7 @@ let get_lts_constructors (x : 'a t) : Rocq_utils.ind_constr array =
 
 (***********************************************************************)
 
-exception
-  Rocq_ind_mip_InconsistentNumConstructors of Declarations.one_inductive_body
+exception Mip_InconsistentNumConstructors of Declarations.one_inductive_body
 
 let mip_to_lts_constructors (mip : Declarations.one_inductive_body)
   : LTS.constructor array
@@ -105,7 +104,7 @@ let mip_to_lts_constructors (mip : Declarations.one_inductive_body)
     |> List.rev
     |> Array.of_list
   with
-  | Invalid_argument _ -> raise (Rocq_ind_mip_InconsistentNumConstructors mip)
+  | Invalid_argument _ -> raise (Mip_InconsistentNumConstructors mip)
 ;;
 
 (***********************************************************************)
