examples/bisimilarity/CADP/Size1/PluginProofs.v
@@ -19,7 +19,7 @@ Require Import Logic.
 
 
 MeBi Divider "Examples.Bisimilarity.CADP.Size1.PluginProofs.bigstep_lts".
-Example wsim_bigstep_lts : weak_sim bigstep lts c1 c1. 
+(* Example wsim_bigstep_lts : weak_sim bigstep lts c1 c1. 
 Proof. MeBi Sim Begin bigstep c1 And lts c1 Using step.
   (* Iteration History: 267 <- 300 <- _ <- _ *) 
   MeBi Sim Solve 267. Qed.
@@ -29,24 +29,43 @@ MeBi Divider "Examples.Bisimilarity.CADP.Size1.PluginProofs.lts_bigstep".
 Example wsim_lts_bigstep : weak_sim lts bigstep c1 c1. 
 Proof. MeBi Sim Begin lts c1 And bigstep c1 Using step. 
   (* Iteration History: 395 <- _ <- _ <- _  *) 
-  MeBi Sim Solve 395. Qed.
+  MeBi Sim Solve 395. Qed. *)
 
 (****************************)
 
-(* TODO: just copied from paper *)
-(* Inductive act' : Type := | ENTER : nat -> nat -> label | LEAVE : nat -> nat -> label. *)
 
 Inductive spec_state : Type :=
-| Free : spec_state
+| Free : nat -> spec_state
 | Held : nat -> spec_state
 .
 
-(* NOTE: needed to add pid *)
 Inductive spec_lts : spec_state -> option label -> spec_state -> Prop :=
-| SVC_ENTER : forall i, spec_lts Free (Some (ENTER, i)) (Held i)
-| SVC_LEAVE : forall i, spec_lts (Held i) (Some (LEAVE, i)) Free
+| SVC_ENTER : forall i, spec_lts (Free i) (Some (ENTER, i)) (Held i)
+| SVC_LEAVE : forall i, spec_lts (Held i) (Some (LEAVE, i)) (Free i)
 .
 
+
+MeBi Divider "Examples.Bisimilarity.CADP.Size1.PluginProofs.lts_spec_lts".
+Example wsim_lts_spec_lts : weak_sim lts spec_lts c1 (Free 0). 
+Proof. MeBi Sim Begin lts c1 And spec_lts (Free 0) Using step.
+  (* Iteration History: _ <- _ <- _ <- _ *) 
+  MeBi Sim Solve 1000. Qed.
+  (* MeBi Sim Solve 68.  *)
+  (* constructor 1. *)
+  (* eauto with rel_db. *)
+
+(* Admitted. *)
+
+  
+MeBi Divider "Examples.Bisimilarity.CADP.Size1.PluginProofs.spec_lts_lts".
+(* Example wsim_spec_lts_lts : weak_sim spec_lts lts (Free 0) c1. 
+Proof. MeBi Sim Begin spec_lts (Free 0) And lts c1 Using step. 
+  (* Iteration History: 207 <- _ <- _ <- _  *) 
+  MeBi Sim Solve 207. Qed. *)
+
+(****************************)
+
+  
 MeBi Divider "Examples.Bisimilarity.CADP.Size1.PluginProofs.bigstep_spec_lts".
 (* Example wsim_bigstep_spec_lts : weak_sim bigstep spec_lts c1 Free. 
 Proof. MeBi Sim Begin bigstep c1 And spec_lts Free Using step.
