examples/CADP_Spec.v
@@ -1,0 +1,105 @@
+Require Import MEBI.Examples.CADP.
+
+From Corelib Require Import Relations.Relation_Definitions.
+From Stdlib Require Import Relations.Relation_Operators.
+From Stdlib Require Operators_Properties.
+
+Require Import MEBI.Bisimilarity.
+
+(* TODO: just copied from paper *)
+(* Inductive act' : Type := | ENTER : nat -> label | LEAVE : nat -> label. *)
+
+Inductive spec_state : Type :=
+| Free : spec_state
+| Held : nat -> spec_state
+.
+
+(* NOTE: needed to add pid *)
+Inductive spec_lts : spec_state -> option label -> spec_state -> Prop :=
+| SVC_ENTER : forall i, spec_lts Free (Some (ENTER, i)) (Held i)
+| SVC_LEAVE : forall i, spec_lts (Held i) (Some (LEAVE, i)) Free
+.
+
+
+Example p1 : tm * env := (Protocol.P, Env.initial 1).
+
+Example c1 : composition := compose (create 1 Protocol.P).
+
+Example d1 : spec_state := Free.
+
+Example wsim_bigstep_spec_lts : weak_sim lts spec_lts c1 d1. 
+Proof. intros. unfold c1, d1. simpl in *. 
+  unfold Resource.initial, State.create.  
+  unfold Vars.initial, Memory.create, Lock.initial. simpl in *.
+  unfold Qnode.initial, Index.initial. 
+  
+  cofix CH0; apply In_sim, Pack_sim; intros.
+  inversion H; subst.
+  inversion H5; subst.
+  simpl in *. clear H H5.
+  exists Free. split; eauto with rel_db.
+
+  cofix CH1; apply In_sim, Pack_sim; intros.
+  inversion H; subst.
+  inversion H5; subst.
+  inversion H4; subst.
+  inversion H6; subst. 
+  simpl in *. clear H H5 H4 H6.
+  exists Free. split; eauto with rel_db.
+  
+  cofix CH2; apply In_sim, Pack_sim; intros.
+  inversion H; subst.
+  inversion H5; subst.
+  inversion H4; subst.
+  - simpl in *. clear H H5 H4.
+    exists Free. split; eauto with rel_db.
+
+    cofix CH3; apply In_sim, Pack_sim; intros.
+    inversion H; subst.
+    inversion H5; subst.
+    inversion H4; subst.
+    inversion H6; subst. 
+    simpl in *. clear H H5 H4 H6.
+    exists Free. split; eauto with rel_db.
+
+    cofix CH4; apply In_sim, Pack_sim; intros.
+    inversion H; subst.
+    inversion H5; subst.
+    inversion H4; subst.
+    * simpl in *. clear H H5 H4.
+      exists Free. split; eauto with rel_db.
+
+      cofix CH5; apply In_sim, Pack_sim; intros.
+      inversion H; subst.
+      inversion H5; subst.
+      inversion H4; subst.
+      simpl in *. clear H H5 H4.
+      exists Free. split; eauto with rel_db.
+      
+      cofix CH6; apply In_sim, Pack_sim; intros.
+      inversion H; subst.
+      inversion H5; subst.
+      simpl in *. clear H H5.
+      + exists Free. split; eauto with rel_db.
+      
+      cofix CH7; apply In_sim, Pack_sim; intros.
+      inversion H; subst.
+      inversion H5; subst.
+      inversion H4; subst.
+      simpl in *. clear H H5 H4.
+      eexists. split.
+      { eapply wk_some; unfold silent.
+        eauto with rel_db. constructor 1.
+        eauto with rel_db. }
+      { 
+        
+      }
+
+
+
+
+Admitted.
+  (* MeBi Sim Begin bigstep c1 And spec_lts Free Using step.
+  (* Iteration History: _ <- _ <- _ <- _ *) 
+  MeBi Sim Solve 1000. Qed. *)
+
